HOL/SepLogic/Union_Find.thy
@@ -1,0 +1,130 @@
+theory Union_Find
+imports "../DataStrs/Union_Find_Func" SepAuto
+begin
+
+type_synonym uf = "nat array \<times> nat array"
+  
+definition is_uf :: "(nat\<times>nat) set \<Rightarrow> uf \<Rightarrow> assn" where
+  "is_uf R u = (\<exists>\<^sub>Al szl. snd u \<mapsto>\<^sub>a l * fst u \<mapsto>\<^sub>a szl *
+        \<up>(ufa_invar l \<and> ufa_\<alpha> l = R \<and> length szl = length l))"
+setup {* add_rewrite_ent_rule @{thm is_uf_def} *}
+
+definition uf_init :: "nat \<Rightarrow> uf Heap" where
+  "uf_init n = do {
+     l \<leftarrow> Array.of_list [0..<n];
+     szl \<leftarrow> Array.new n (1::nat);
+     return (szl, l)
+   }"
+declare uf_init_def [sep_proc_defs]
+
+lemma triv_equiv_rel_iff [rewrite]:
+  "(x,y) \<in> {(i,i) |i. i<n} \<longleftrightarrow> (x = y \<and> x < n)" by blast
+
+lemma uf_init_rule [hoare_triple]:
+  "<emp> uf_init n <is_uf {(i,i) |i. i<n}>" by auto2
+declare uf_init_def [sep_proc_defs del]
+  
+partial_function (heap) uf_rep_of :: "nat array \<Rightarrow> nat \<Rightarrow> nat Heap" where [code]: 
+  "uf_rep_of p i = do {
+     n \<leftarrow> Array.nth p i;
+     if n = i then return i else uf_rep_of p n
+   }"
+declare uf_rep_of.simps [sep_proc_defs]
+  
+lemma uf_rep_of_rule [hoare_triple]:
+  "<p \<mapsto>\<^sub>a l * \<up>(ufa_invar l) * \<up>(i < length l)>
+   uf_rep_of p i
+   <\<lambda>r. p \<mapsto>\<^sub>a l * \<up>(r = rep_of l i)>"
+@proof @contradiction
+  @prop_induct "ufa_invar l \<and> i < length l"
+    "<p \<mapsto>\<^sub>a l * \<up>(ufa_invar l) * \<up>(i < length l)>
+     uf_rep_of p i
+     <\<lambda>r. p \<mapsto>\<^sub>a l * \<up>(r = rep_of l i)>"
+@qed
+declare uf_rep_of.simps [sep_proc_defs]
+
+partial_function (heap) uf_compress :: "nat \<Rightarrow> nat \<Rightarrow> nat array \<Rightarrow> unit Heap" where [code]: 
+  "uf_compress i ci p = (
+    if i = ci then return ()
+    else do {
+      ni \<leftarrow> Array.nth p i;
+      uf_compress ni ci p;
+      Array.upd i ci p;
+      return ()
+    })"
+declare uf_compress.simps [sep_proc_defs]
+
+lemma uf_compress_rule [hoare_triple]:
+  "<p \<mapsto>\<^sub>a l * \<up>(ufa_invar l) * \<up>(i < length l) * \<up>(ci = rep_of l i)>
+   uf_compress i ci p
+   <\<lambda>_. \<exists>\<^sub>Al'. p \<mapsto>\<^sub>a l' * \<up>(ufa_invar l' \<and> length l' = length l \<and> (\<forall>i<length l. rep_of l' i = rep_of l i))>"
+@proof @contradiction
+  @prop_induct "ufa_invar l \<and> i < length l"
+    "<p \<mapsto>\<^sub>a l * \<up>(ufa_invar l) * \<up>(i < length l) * \<up>(ci = rep_of l i)>
+     uf_compress i ci p
+     <\<lambda>_. \<exists>\<^sub>Al'. p \<mapsto>\<^sub>a l' * \<up>(ufa_invar l' \<and> length l' = length l \<and> (\<forall>i<length l. rep_of l' i = rep_of l i))>"
+@qed
+declare uf_compress.simps [sep_proc_defs del]
+
+definition uf_rep_of_c :: "nat array \<Rightarrow> nat \<Rightarrow> nat Heap" where
+  "uf_rep_of_c p i = do {
+    ci \<leftarrow> uf_rep_of p i;
+    uf_compress i ci p;
+    return ci
+  }"
+declare uf_rep_of_c_def [sep_proc_defs]
+
+lemma uf_rep_of_c_rule [hoare_triple]:
+  "<p \<mapsto>\<^sub>a l * \<up>(ufa_invar l) * \<up>(i < length l)>
+   uf_rep_of_c p i
+   <\<lambda>r. \<exists>\<^sub>Al'. p \<mapsto>\<^sub>a l' * \<up>(r = rep_of l i \<and> ufa_invar l' \<and> length l' = length l \<and>
+                          (\<forall>i<length l. rep_of l' i = rep_of l i))>"
+  by auto2
+declare uf_rep_of_c_def [sep_proc_defs del]
+
+definition uf_cmp :: "uf \<Rightarrow> nat \<Rightarrow> nat \<Rightarrow> bool Heap" where 
+  "uf_cmp u i j \<equiv> do {
+    n \<leftarrow> Array.len (snd u);
+    if (i\<ge>n \<or> j\<ge>n) then return False
+    else do {
+      ci \<leftarrow> uf_rep_of_c (snd u) i;
+      cj \<leftarrow> uf_rep_of_c (snd u) j;
+      return (ci = cj)
+    }
+  }"
+declare uf_cmp_def [sep_proc_defs]
+
+lemma uf_cmp_rule [hoare_triple]:
+  "<is_uf R u>
+   uf_cmp u i j
+   <\<lambda>r. is_uf R u * \<up>(r \<longleftrightarrow> (i,j)\<in>R)>" by auto2
+declare uf_cmp_def [sep_proc_defs del]
+
+definition uf_union :: "uf \<Rightarrow> nat \<Rightarrow> nat \<Rightarrow> uf Heap" where 
+  "uf_union u i j \<equiv> do {
+    ci \<leftarrow> uf_rep_of (snd u) i;
+    cj \<leftarrow> uf_rep_of (snd u) j;
+    if (ci = cj) then return u
+    else do {
+      si \<leftarrow> Array.nth (fst u) ci;
+      sj \<leftarrow> Array.nth (fst u) cj;
+      if si < sj then do {
+        Array.upd ci cj (snd u);
+        Array.upd cj (si+sj) (fst u);
+        return u
+      } else do { 
+        Array.upd cj ci (snd u);
+        Array.upd ci (si+sj) (fst u);
+        return u
+      }
+    }
+  }"
+declare uf_union_def [sep_proc_defs]
+
+lemma uf_union_rule:
+  "<is_uf R u * \<up>(i \<in> Domain R) * \<up>(j \<in> Domain R)>
+   uf_union u i j
+   <is_uf (per_union R i j)>" by auto2
+declare uf_union_def [sep_proc_defs del]
+
+end
